fixed TyVar so that we can prove the elam inversion (had an admit in the previous version. essestially made it to that typing judgments yield types that have KTyp kind

examples/metatheory/lambda_omega.fst
@@ -299,6 +299,7 @@ type tequiv : typ -> typ -> Type =
 type typing : env -> exp -> typ -> Type =
   | TyVar : #g:env ->
             x:var{is_Some (lookup_evar g x)} ->
+            kinding g (Some.v (lookup_evar g x)) KTyp ->
             typing g (EVar x) (Some.v (lookup_evar g x))
   | TyLam : #g:env ->
             t:typ ->
@@ -437,7 +438,7 @@ val econtext_invariance : #e:exp -> #g:env -> #t:typ ->
       Tot (typing g' e t) (decreases h)
 let rec econtext_invariance _ _ t h g' =
   match h with
-    | TyVar x -> TyVar x
+    | TyVar x h -> TyVar x (kinding_extensional h g')
     | TyLam #g t_y #e1 #t' hk h1 ->
       TyLam t_y (tcontext_invariance hk g')
   	(econtext_invariance #e1 #(extend_evar g 0 t_y) #t' h1
@@ -445,6 +446,7 @@ let rec econtext_invariance _ _ t h g' =
     | TyApp h1 h2 -> TyApp (econtext_invariance h1 g')
                            (econtext_invariance h2 g')
     | TyEqu h1 eq k -> TyEqu (econtext_invariance h1 g') eq (kinding_extensional k g')
+
 
 (* kinding weakening when a term variable binding is added to env *)
 val kinding_weakening_ebnd : #g:env -> #t:typ -> #k:knd ->
@@ -503,6 +505,23 @@ val kinding_strengthening_ebnd : g:env -> x:var -> t_x:typ -> #t:typ -> #k:knd -
       Tot (kinding g t k) (decreases h)
 let kinding_strengthening_ebnd g x t_x t k h = kinding_extensional h g
 
+val kinding_inversion_arrow: #g:env -> #t1:typ -> #t2:typ ->
+                             h:(kinding g (TArr t1 t2) KTyp) ->
+                             Tot (cand (kinding g t1 KTyp) (kinding g t2 KTyp))
+let rec kinding_inversion_arrow g t1 t2 h = match h with
+  | KiArr h1 h2 -> Conj h1 h2
+
+val typing_gives_well_kinded_types: #g:env -> #e:exp -> #t:typ ->
+                                    h:(typing g e t) ->
+                                    Tot (kinding g t KTyp) (decreases h)
+let rec typing_gives_well_kinded_types g e t h = match h with
+  | TyVar x h -> h
+  | TyLam t' hk h1 -> KiArr hk (kinding_strengthening_ebnd g 0 t' (typing_gives_well_kinded_types h1))
+  | TyApp #g #e1 #e2 #t1 #t2 h1 h2 ->
+    let Conj pa pb = kinding_inversion_arrow #g #t1 #t2 (typing_gives_well_kinded_types h1) in
+    pb
+  | TyEqu h1 eq hk -> hk
+
 (* this folows from functional extensionality *)
 val typing_extensional: #g:env -> #e:exp -> #t:typ -> h:(typing g e t) ->
                 g':env{FEq (MkEnv.x g) (MkEnv.x g') /\
@@ -516,7 +535,9 @@ val typing_weakening_ebnd: #g:env -> x:var -> t_x:typ -> #e:exp -> #t:typ ->
                                       (eshift_up_above x e) t) (decreases h)
 let rec typing_weakening_ebnd g x t_x e t h =
   match h with
-    | TyVar y -> if y < x then TyVar y else TyVar (y+1)
+    | TyVar y h ->
+      let h1 = kinding_weakening_ebnd h x t_x in
+      if y < x then TyVar y h1 else TyVar (y+1) h1
     | TyLam #g t_y #e' #t'' kh h21 ->
       eshift_up_above_lam x t_y e';
       let h21 = typing_weakening_ebnd (x+1) t_x h21 in
@@ -593,7 +614,7 @@ val typing_weakening_tbnd: #g:env -> x:var -> k_x:knd -> #e:exp -> #t:typ ->
                   (tshift_up_above_e x e) (tshift_up_above x t)) (decreases h)
 let rec typing_weakening_tbnd g x k_x e t h =
   match h with
-    | TyVar y -> TyVar y
+    | TyVar y h -> TyVar y (kinding_weakening_tbnd h x k_x)
     | TyLam #g t' #e1 #t'' kh h1 ->
       TyLam (tshift_up_above x t') (kinding_weakening_tbnd kh x k_x)
             (typing_extensional (typing_weakening_tbnd x k_x h1)
@@ -616,9 +637,11 @@ val typing_substitution: x:nat -> #e:exp -> #v:exp -> #t_x:typ -> #t:typ ->
       Tot (typing g (esubst_beta_gen x v e) t) (decreases %[e;h2])
 let rec typing_substitution x e v t_x t g h1 h2 =
   match h2 with
-    | TyVar y -> if x = y then h1
+    | TyVar y hk ->
+      (*let hk1 = kinding_strengthening_ebnd g x t_x t KTyp hk in*)
+      if x = y then h1
       else if y < x then econtext_invariance h2 g
-      else TyVar (y - 1)
+      else TyVar (y - 1) (kinding_strengthening_ebnd g x t_x hk)
     | TyLam #g' t_y #e' #t' kh h21 ->
       let h21' = typing_extensional h21 (extend_evar (extend_evar g 0 t_y) (x+1) t_x) in
       let h1' = typing_weakening_ebnd 0 t_y h1 in
@@ -1037,18 +1060,36 @@ let rec inversion_elam g s1 e s t1 t2 ht heq = match ht with
     let Conj ptu1 ptu2 = p in
     
     (*
-     * AR: this I think is a hole in TAPL proof ? we have nothing in the
-     * context to show that t2 has kind KTyp in g. one way to get this is
-     * to ensure that typing judgments result in KTyp kinded types. then,
-     * we can argue that s2 is KTyp in g and so, since s2 equiv t2, t2 
-     * has KTyp kind in g. but to show that all typing judgments result in
-     * KTyp kinded types, we need to fix TyVar rule and add a check there.
+     * AR: so now we have tequiv s2 t2, and ht1. as TAPL says, we now want to use
+     * TyEqu to derive typing judgment with result type t2 (ht1 has result type s2).
+     * but, TyEqu also requires that g |- t2 :: KTyp, which means we are stuck.
+     * i don't see a way to derive this kinding judgment just given the premises.
+     * 
+     * i am fixing it by making sure that all typing judgments result in types
+     * that have kind KTyp. so then, we can derive s2::KTyp, and since tequiv s2 t2,
+     * we will get t2::KTyp. to do so, i had to make a small change to TyVar
+     * requiring that the lookup type has kind KTyp.
      *)
-       
+    
+    (*
+     * AR: the code below is somewhat unstable. for example, removing type annotations
+     * fails verification, without an unnecessary admit below, the verification
+     * fails, cannot use Conj.pb directly, have to let bind.
+     *)
+           
+    (* AR: removing this type annotation, verification fails after taking a long time *)
+    let d1:(cand (kinding g s1 KTyp) (kinding g s2 KTyp)) =
+      kinding_inversion_arrow (typing_gives_well_kinded_types ht) in
+    let Conj pa pb = d1 in
+
+    let pst2 = EqTran (tred_star_tequiv psu2) (EqSymm (tred_star_tequiv ptu2)) in
+    let Conj paa pbb = kinding_tequiv pst2 in
+        
+    let h'':(kinding g t2 KTyp) = paa pb in
+    (* AR: without this unnecessary admit below, verification fails ... why should it matter. note that we have h'' on the previous line with same type, so we don't need this admit ? *)
     let h'':(kinding g t2 KTyp) = admit () in
 
-    Conj (EqTran (tred_star_tequiv ptu1) (EqSymm (tred_star_tequiv psu1)))
-         (TyEqu ht1 (EqTran (tred_star_tequiv psu2) (EqSymm (tred_star_tequiv ptu2))) h'')
+    Conj (EqTran (tred_star_tequiv ptu1) (EqSymm (tred_star_tequiv psu1))) (TyEqu ht1 pst2 h'')
 
 (* corollary of inversion_elam *)
 val inversion_elam_typing : #g:env -> s1:typ -> e:exp ->
